proof: the weight of a childfree node is 1

proofs.v
@@ -1,43 +1,68 @@
-Check 3.
-Check 1+2.
-Check True.
-Check False.
-Check (3=5).
-Check (3, 5).
-Check ((3=6)/\False).
-Check nat:Set.
-Check nat:Type.
-Check nat -> Prop.
-Check 3 <= 5.
-  Check (forall x:nat, x < 3 \/ (exists y:nat, x = y + 3)).
-Check (and True).
-Check (and True True).
-Eval compute in let f := fun x => (x + 1, x) in f 1.
+Set Printing Projections.
+Require Import Bool.
+Require Import List.
 Inductive Correctness : Type :=
   | yes : Correctness
   | no : Correctness
   | trusted : Correctness
 | idk : Correctness.
-Check yes.
-Check no.
-Require Import List.
+Example yes_is_yes : yes = yes.
+Proof. reflexivity.
+Qed.
+Example no_is_no : no = no.
+Proof. reflexivity.
+Qed.
+Example trusted_is_trusted : trusted = trusted.
+Proof. reflexivity.
+Qed.
+Example idk_is_idk : idk = idk.
+Proof. reflexivity.
+Qed.
+
 Inductive Node : Type := mkNode
- { node_correctness : Correctness
+ { correctness : Correctness
  ; children : list Node
  }.
+(* Inductive DebuggingTree : Type := *)
+(*     right_neutral : forall x, x * 1 = x  *)
 Definition node1 := mkNode idk nil.
 Definition node2 := mkNode idk nil.
-Definition node3 := mkNode idk (node1::node2::nil).
-Set Printing Projections.
-Fixpoint sum_list l : nat :=
+Definition node3 := mkNode trusted (node1::node2::nil).
+Eval compute in correctness node3.
+Fixpoint sum_list (l : list nat) : nat :=
   match l with
     nil => 0
   | n::tl => n + sum_list tl
   end.
+Fixpoint and_list (l : list bool) : bool :=
+  match l with
+    nil => true
+  | n::tl => andb n (and_list tl)
+  end.
+Eval compute in and_list (true::true::true::nil).
+Search bool.
+Check 1::nil.
 Fixpoint weight (node : Node) : nat :=
   match node.(children) with
     nil => 1
-  | children => 1 + sum_list (map (fun my_child => weight my_child) (children))
+  | children => 1 + sum_list (map (fun child => weight child) (children))
   end.
+Lemma commutativity : forall a b:Prop, a/\b -> b/\a.
+Proof.
+  intros a b H. split. destruct H as [H1 H2]. exact H2. intuition.
+  Qed.
+Lemma weight_childfree_node_eq_1: forall n:Node, n.(children) = nil -> weight n = 1.
+Proof.
+  - intros n H. induction n. simpl. assert (children0 = nil). apply H. subst. reflexivity.
+Qed.
+Lemma weight_ge_1: forall n:Node, weight n > 0.
+Proof. intros. induction n. induction children0.
+Eval compute in idk = idk.
+Fixpoint are_all_idk (node : Node) : bool :=
+  match node.(children) with
+    nil => eqb (node.(correctness) idk)
+  | children => eqb node.(correctness) (andb idk (and_list (map (fun child => are_all_idk child) (children))))
+  end.
+Check are_all_idk node3.
 Eval compute in sum_list (map (fun x => x + 3) (1::2::5::nil)).
-Eval compute in weight node1.
+Eval compute in weight node3.
